Checkpoint

new-semantics/coq/.CoqMakefile.d
@@ -13,9 +13,9 @@ theories/EnvSemantics.vos theories/EnvSemantics.vok theories/EnvSemantics.requir
 theories/EquivFacts.vo theories/EquivFacts.glob theories/EquivFacts.v.beautified theories/EquivFacts.required_vo: theories/EquivFacts.v basics/Basics.vo theories/Defs.vo theories/SubstFacts.vo
 theories/EquivFacts.vio: theories/EquivFacts.v basics/Basics.vio theories/Defs.vio theories/SubstFacts.vio
 theories/EquivFacts.vos theories/EquivFacts.vok theories/EquivFacts.required_vos: theories/EquivFacts.v basics/Basics.vos theories/Defs.vos theories/SubstFacts.vos
-theories/MemSemantics.vo theories/MemSemantics.glob theories/MemSemantics.v.beautified theories/MemSemantics.required_vo: theories/MemSemantics.v 
-theories/MemSemantics.vio: theories/MemSemantics.v 
-theories/MemSemantics.vos theories/MemSemantics.vok theories/MemSemantics.required_vos: theories/MemSemantics.v 
+theories/MemSemantics.vo theories/MemSemantics.glob theories/MemSemantics.v.beautified theories/MemSemantics.required_vo: theories/MemSemantics.v basics/Basics.vo theories/Defs.vo theories/Syntax.vo theories/SubstFacts.vo theories/EnvSemantics.vo
+theories/MemSemantics.vio: theories/MemSemantics.v basics/Basics.vio theories/Defs.vio theories/Syntax.vio theories/SubstFacts.vio theories/EnvSemantics.vio
+theories/MemSemantics.vos theories/MemSemantics.vok theories/MemSemantics.required_vos: theories/MemSemantics.v basics/Basics.vos theories/Defs.vos theories/Syntax.vos theories/SubstFacts.vos theories/EnvSemantics.vos
 theories/SubstFacts.vo theories/SubstFacts.glob theories/SubstFacts.v.beautified theories/SubstFacts.required_vo: theories/SubstFacts.v basics/Basics.vo theories/Defs.vo
 theories/SubstFacts.vio: theories/SubstFacts.v basics/Basics.vio theories/Defs.vio
 theories/SubstFacts.vos theories/SubstFacts.vok theories/SubstFacts.required_vos: theories/SubstFacts.v basics/Basics.vos theories/Defs.vos
