new-semantics/coq/theories/MemSemantics.v
@@ -1,0 +1,224 @@
+From Basics Require Import Basics.
+From LN Require Import Defs.
+From LN Require Import Syntax.
+From LN Require Import SubstFacts.
+From LN Require Import EnvSemantics.
+
+Fixpoint read_menv {var loc} `{Eq var} (σ : menv var loc) (x : var) :=
+  match σ with
+  | [] => None
+  | (x', ℓ) :: σ' =>
+    if eqb x x' then Some ℓ else read_menv σ' x
+  end.
+
+Inductive meval {var loc} `{Eq var} `{Eq loc} (σ : menv var loc) (m : memory var loc val) (L : list loc) :
+  (@tm var) -> (mvalue var loc (@val var)) -> (memory var loc (@val var)) -> list loc -> Prop :=
+| mev_id x ℓ v
+  (READσ : read_menv σ x = Some ℓ)
+  (READm : m ℓ = Some v)
+: meval σ m L (tm_var x) v m L
+| mev_fn x t
+: meval σ m L (tm_lam x t) (mvalue_clos (v_fn x t) σ) m L
+| mev_app t1 t2 x t σ1 m1 L1 v2 m2 L2 ℓ v m' L'
+  (FN : meval σ m L t1 (mvalue_clos (v_fn x t) σ1) m1 L1)
+  (ARG : meval σ m1 L1 t2 v2 m2 L2)
+  (DOMm : m2 ℓ = None)
+  (DOML : ~ In ℓ L2)
+  (BODY : meval ((x, ℓ) :: σ1) (ℓ !-> v2 ; m2) L2 t v m' L')
+: meval σ m L (tm_app t1 t2) v m' L'
+| mev_link t1 t2 σ1 m1 L1 v m' L'
+  (MOD : meval σ m L t1 (mvalue_exp σ1) m1 L1)
+  (IMP : meval σ1 m1 L1 t2 v m' L')
+: meval σ m L (tm_link t1 t2) v m' L'
+| mev_mt
+: meval σ m L tm_mt (mvalue_exp []) m L
+| mev_bind x t1 t2 ℓ v1 m1 L1 σ2 m' L'
+  (DOM : m ℓ = None)
+  (FRESH : ~ In ℓ L)
+  (BIND : meval ((x, ℓ) :: σ) m (ℓ :: L) t1 v1 m1 L1)
+  (MOD : meval ((x, ℓ) :: σ) (ℓ !-> v1 ; m1) L1 t2 (mvalue_exp σ2) m' L')
+: meval σ m L (tm_bind x t1 t2) (mvalue_exp ((x, ℓ) :: σ2)) m' L'
+.
+
+Fixpoint distinct {T} (l : list T) :=
+  match l with
+  | [] => True
+  | hd :: tl => ~ In hd tl /\ distinct tl
+  end.
+
+Fixpoint delete {T} `{Eq T} (l : list T) (t : T) :=
+  match l with
+  | [] => []
+  | hd :: tl =>
+    if eqb t hd then delete tl t else hd :: (delete tl t)
+  end.
+
+Fixpoint diff {T} `{Eq T} (a b : list T) :=
+  match b with
+  | [] => a
+  | hd :: tl => diff (delete a hd) tl
+  end.
+
+Lemma delete_in {T} `{Eq T} (l : list T) :
+  forall x ℓ,
+    In ℓ (delete l x) <-> In ℓ l /\ ℓ <> x.
+Proof.
+  induction l; ii; ss. tauto.
+  des_ifs; eqb2eq T; ss; clarify.
+  firstorder. contradict.
+  firstorder. clarify. auto.
+Qed.
+
+Lemma delete_distinct {T} `{Eq T} (l : list T) :
+  forall x (DIST : distinct l), distinct (delete l x).
+Proof.
+  induction l; ii; ss. des.
+  des_ifs; eqb2eq T; clarify; ss; eauto.
+  split; eauto.
+  ii. rewrite delete_in in *. des; clarify.
+Qed. 
+
+Lemma delete_free {T} `{Eq T} (l : list T) :
+  forall x (nIN : ~ In x l),
+    delete l x = l.
+Proof.
+  induction l; ii; ss.
+  split_nIn. des_ifs; eqb2eq T; clarify.
+  rw; eauto.
+Qed.
+
+Lemma delete_len {T} `{Eq T} (l : list T) :
+  forall x (DIST : distinct l),
+    length l - 1 <= length (delete l x).
+Proof.
+  induction l; ii; ss.
+  des; des_ifs; eqb2eq T; clarify.
+  rewrite delete_free; eauto. nia.
+  s. exploit IHl; eauto. instantiate (1 := x).
+  nia.
+Qed.
+
+Lemma diff_in {T} `{Eq T} (b : list T) :
+  forall a x,
+    In x (diff a b) <-> In x a /\ ~ In x b.
+Proof.
+  induction b; ii; ss. tauto.
+  rw. rewrite delete_in. firstorder.
+Qed.
+
+Lemma diff_len {T} `{Eq T} (b : list T) :
+  forall a (DIST : distinct a) (LE : length b <= length a),
+    length a - length b <= length (diff a b).
+Proof.
+  induction b; ii; ss. nia.
+  eapply delete_len with (x := a) in DIST as LEN.
+  exploit (IHb (delete a0 a)).
+  apply delete_distinct.
+  all: first [nia | auto].
+Qed.
+
+Lemma list_spill {T} `{Eq T} :
+  forall (a b : list T) (LEN : length a < length b)
+    (DISb : distinct b),
+  exists x, In x b /\ ~ In x a.
+Proof.
+  ii. remember (diff b a) as l.
+  exploit (diff_len a b DISb). nia.
+  rrw. destruct l; ii; ss. nia.
+  exists t. apply diff_in. rrw. s. auto.
+Qed.
+
+Lemma map_distinct {loc} `{Eq loc} (l : list loc) :
+  forall (DIST : distinct l) (f : loc -> loc) (INJ : forall ℓ ν (fEQ : f ℓ = f ν), ℓ = ν),
+    distinct (map f l).
+Proof.
+  induction l; ii; ss.
+  des. split; eauto.
+  red. intros IN. clear DIST0 IHl.
+  ginduction l; ii; ss; split_nIn; des; clarify.
+  apply INJ in IN. clarify.
+  exploit IHl; eauto.
+Qed.
+
+Lemma map_in {loc} `{Eq loc} (l : list loc) :
+  forall y (f : loc -> loc) (INJ : forall ℓ ν (fEQ : f ℓ = f ν), ℓ = ν) (IN : In y (map f l)),
+    exists x, In x l /\ f x = y.
+Proof.
+  induction l; ii; ss; des; clarify; eauto.
+  exploit IHl; eauto. ii; des; eauto.
+Qed.
+
+Fixpoint genlist {loc} `{Name loc} L n :=
+  match n with
+  | 0 => []
+  | S n' =>
+    let L' := genlist L n' in
+    let ℓ := gensym (L' ++ L) in
+    ℓ :: L'
+  end.
+
+Lemma genlist_length {loc} `{Name loc} n :
+  forall L, length (genlist L n) = n.
+Proof.
+  induction n; ii; ss. rw. eauto.
+Qed.
+
+Lemma genlist_distinct {loc} `{Name loc} n :
+  forall L, distinct (genlist L n).
+Proof.
+  induction n; ii; ss. split; auto.
+  ii. exploit gensym_spec; eauto.
+  instantiate (1 := genlist L n ++ L).
+  rewrite in_app_iff. auto.
+Qed.
+
+Lemma genlist_avoid {loc} `{Name loc} n :
+  forall L x (IN : In x (genlist L n)), ~ In x L.
+Proof.
+  induction n; ii; ss. des; eauto.
+  exploit gensym_spec; eauto.
+  instantiate (1 := genlist L n ++ L). rw.
+  rewrite in_app_iff; auto.
+  exploit IHn; eauto.
+Qed.
+
+Lemma avoid_dom_ran {loc} `{Name loc} L :
+  forall L' (f : loc -> loc) (INJ : forall ℓ ν (fEQ : f ℓ = f ν), ℓ = ν),
+    exists x, ~ In x L /\ ~ In (f x) L'.
+Proof.
+  ii. remember (genlist L (1 + length L')) as l.
+  exploit (list_spill L' (map f l)).
+  rewrite map_length. rw. rewrite genlist_length. auto.
+  apply map_distinct; auto. rw. apply genlist_distinct.
+  ii; des. exploit map_in; eauto.
+  rw. intros (x' & IN' & EQ').
+  apply genlist_avoid in IN'.
+  exists x'. rw. eauto.
+Qed.
+
+Definition fin {A B} (f : A -> option B) :=
+  exists dom, forall x (fDOM : ~ In x dom), f x = None.
+
+Definition bot {A B} : A -> option B := fun x => None.
+
+Definition Equiv {var loc} `{Eq var} `{Eq loc} (w : wvl var loc (@val var)) W m L :=
+  equiv w bot W m /\ (forall ℓ (IN : In ℓ (floc_wvl w)), In ℓ L).
+
+#[local] Coercion vl_exp : nv >-> vl.
+#[local] Coercion wvl_v : vl >-> wvl.
+
+Lemma equiv_l {var loc} `{Eq var} `{Name loc} (σ : nv var loc val) t v (EVAL : eval σ t v) :
+  forall φ σ' m L
+    (INJ : forall x y (fEQ : φ x = φ y), x = y)
+    (EQUIV : Equiv (map_nv φ σ) (mvalue_exp σ') m L) (FIN : fin m),
+    exists v' m' L',
+      (meval σ' m L t v' m' (L' ++ L)) /\
+      (Equiv (map_vl φ v) v' m' (L' ++ L)) /\
+      (fin m') /\
+      (forall ℓ (INℓ : In ℓ L), m' ℓ = m ℓ) /\
+      (forall ℓ (DOM : m ℓ <> None), m' ℓ = m ℓ).
+Proof.
+  induction EVAL; ii; ss.
+Admitted.
+
+ 
